proofmode/HTactics.v
@@ -229,8 +229,8 @@ Section HLEMMAS.
 
         (WEAKER: fspec_weaker fsp1 fsp0)
 
-        ctx0 I
-        (ACC: current_iProp ctx0 I)
+        fr0 I
+        (ACC: current_iProp (fr0 ⋅ mr_src0) I)
 
         (UPDATABLE:
            I ⊢ #=> (FR ** R a0 mp_src0 mp_tgt0 ** (fsp1.(precond) x varg_src varg_tgt: iProp)))
@@ -241,42 +241,46 @@ Section HLEMMAS.
         (POST: forall (vret_tgt : Any.t) (mr_src1: Σ) (mp_src1 mp_tgt1: Any.t) a1
                       (vret_src: Any.t)
                       (WLE: le a0 a1)
-                      ctx1
-                      (ACC: current_iProp ctx1 (FR ** R a1 mp_src1 mp_tgt1 ** fsp1.(postcond) x vret_src vret_tgt))
+                      fr1
+                      (ACC: current_iProp (fr1 ⋅ mr_src1) (FR ** R a1 mp_src1 mp_tgt1 ** fsp1.(postcond) x vret_src vret_tgt))
           ,
                 gpaco8 (_sim_itree (mk_wf R) le fl_src fl_tgt) (cpn8 (_sim_itree (mk_wf R) le fl_src fl_tgt)) rg rg _ _ eqr true true a
-                  (Any.pair mp_src1 mr_src1↑, k_src (ctx1, vret_src)) (mp_tgt1, k_tgt vret_tgt))
+                  (Any.pair mp_src1 mr_src1↑, k_src (fr1, vret_src)) (mp_tgt1, k_tgt vret_tgt))
                 :
       gpaco8 (_sim_itree (mk_wf R) le fl_src fl_tgt) (cpn8 (_sim_itree (mk_wf R) le fl_src fl_tgt)) r rg _ _ eqr m n a
-             (Any.pair mp_src0 mr_src0, (HoareCall tbr ord_cur fsp0 fn varg_src) ctx0 >>= k_src)
+             (Any.pair mp_src0 mr_src0↑, (HoareCall tbr ord_cur fsp0 fn varg_src) fr0 >>= k_src)
              (mp_tgt0, trigger (Call fn varg_tgt) >>= k_tgt)
   .
   Proof.
-    subst. unfold HoareCall, ASSUME, ASSERT, mput, mget, assume, guarantee.
+    subst. unfold HoareCall, mput, mget, assume, guarantee.
     ired_both. apply sim_itreeC_spec. econs 8.
     hexploit (WEAKER x). i. des.
     assert (exists mr_src0' rarg_src fr_src0',
-               (<<UPDATABLE: URA.wf (ctx0 ⋅ (mr_src0' ⋅ (rarg_src ⋅ fr_src0')))>>) /\
+               (<<UPDATABLE: URA.updatable (fr0 ⋅ mr_src0) (mr_src0' ⋅ (rarg_src ⋅ fr_src0'))>>) /\
                (<<RSRC: R a0 mp_src0 mp_tgt0 mr_src0'>>) /\
                (<<FRS: FR fr_src0'>>) /\
                (<<PRE: fsp0.(precond) x_tgt varg_src varg_tgt rarg_src>>)).
-    { inv ACC. uipropall. hexploit UPDATABLE.
-      { eapply URA.wf_mon. eapply GWF. }
-      { eapply IPROP. }
-      { et. }
+    { inv ACC. uipropall. 
+      hexploit UPDATABLE; try apply IPROP.
+      { eapply URA.updatable_wf; et. }
       i. des. subst.
-      hexploit PRE; et. i. uipropall. hexploit (H0 b); et.
-      { eapply URA.wf_mon in H. rewrite URA.add_comm in H. eapply URA.wf_mon in H. auto. }
-      { instantiate (1:=a2 ⋅ b0 ⋅ ctx0).
-        replace (b ⋅ (a2 ⋅ b0 ⋅ ctx0)) with (a2 ⋅ b0 ⋅ b ⋅ ctx0); auto. r_solve. }
-      i. des. esplits; et.
-      { replace (ctx0 ⋅ (b0 ⋅ (r1 ⋅ a2))) with (r1 ⋅ (a2 ⋅ b0 ⋅ ctx0)); auto. r_solve. }
+      hexploit PRE; et. i. uipropall. 
+      hexploit (H b); et.
+      { eapply URA.updatable_wf; et. etrans; et. etrans; et. eapply URA.extends_updatable.
+        exists (a2 ⋅ b0). r_solve. }
+      i; des.
+      esplits; et.
+      etrans; et. etrans; et.
+        replace (b0 ⋅ (r1 ⋅ a2)) with (b0 ⋅ a2 ⋅ r1) by r_solve.
+      eapply URA.updatable_add; et. rewrite URA.add_comm; ss.
     }
-    des. exists x_tgt.
-    repeat (ired_both; apply sim_itreeC_spec; econs 8). exists (rarg_src, fr_src0', mr_src0').
-    repeat (ired_both; apply sim_itreeC_spec; econs 12).
+    des. exists (rarg_src, fr_src0', mr_src0').
+    repeat (ired_both; apply sim_itreeC_spec; econs 12). s. rewrite Any.pair_split.
     repeat (ired_both; apply sim_itreeC_spec; econs 8). unshelve esplits; eauto.
-    { r_wf UPDATABLE0. }
+    { replace (rarg_src ⋅ fr_src0' ⋅ mr_src0') with (mr_src0' ⋅ (rarg_src ⋅ fr_src0')) by r_solve. ss. }
+
+    repeat (ired_both; apply sim_itreeC_spec; econs 12).
+    repeat (ired_both; apply sim_itreeC_spec; econs 8). exists x_tgt.
     repeat (ired_both; apply sim_itreeC_spec; econs 8). exists varg_tgt.
     repeat (ired_both; apply sim_itreeC_spec; econs 8). unshelve esplits; eauto.
     repeat (ired_both; apply sim_itreeC_spec; econs 8). unshelve esplits; eauto.
@@ -285,20 +289,20 @@ Section HLEMMAS.
     { i. spc PURE1. r in MEASURE. des_ifs; ss; des_ifs. }
     repeat (ired_both; apply sim_itreeC_spec; econs).
     { econs; eauto. }
-    i. repeat (ired_both; apply sim_itreeC_spec; econs). i. destruct x0.
+    i. repeat (ired_both; apply sim_itreeC_spec; econs). i. 
     repeat (ired_both; apply sim_itreeC_spec; econs). inv WF.
     repeat (ired_both; apply sim_itreeC_spec; econs). i.
     repeat (ired_both; apply sim_itreeC_spec; econs). i.
     repeat (ired_both; apply sim_itreeC_spec; econs). i. 
     ired_both. eapply POST; eauto. hexploit POST0. i.
-    uipropall. hexploit (H c); et.
-    { eapply URA.wf_mon. instantiate (1:=fr_src0' ⋅ c0 ⋅ mr_src). r_wf x0. }
-    { instantiate (1:=fr_src0' ⋅ c0 ⋅ mr_src). r_wf x0. }
+    uipropall. hexploit (H x0); et.
+    { eapply URA.wf_extends; et. exists (fr_src0' ⋅ mr_src). r_solve. }
     i. des. econs.
-    { instantiate (1:=fr_src0' ⋅ mr_src ⋅ r1). r_wf H0. }
-    red. esplits; et.
-    eapply RSRC0.
-    eapply URA.wf_mon. instantiate (1:=r1 ⋅ fr_src0' ⋅ c0). r_wf H0.
+    { cbn. esplits; et. eapply RSRC0; et. eapply URA.wf_extends; et. exists (fr_src0' ⋅ x0). r_solve. }
+    { ss. }
+    replace (fr_src0' ⋅ mr_src ⋅ r1) with (r1 ⋅ fr_src0' ⋅ mr_src) by r_solve.
+    rewrite <- ! URA.add_assoc.
+    eapply URA.updatable_add; et. refl.
   Qed.
 
   Lemma hcall_clo_ord_weaken
@@ -317,8 +321,8 @@ Section HLEMMAS.
 
         (WEAKER: fspec_weaker fsp1 fsp0)
 
-        ctx0 l
-        (ACC: current_iPropL ctx0 l)
+        fr0 l
+        (ACC: current_iPropL (fr0 ⋅ mr_src0) l)
 
         (UPDATABLE:
            from_iPropL (fst (alist_pops Hns l)) ⊢ #=> (R a0 mp_src0 mp_tgt0 ** (fsp1.(precond) x varg_src varg_tgt: iProp)))
@@ -329,14 +333,14 @@ Section HLEMMAS.
         (POST: forall (vret_tgt : Any.t) (mr_src1: Σ) mp_src1 mp_tgt1 a1
                       (vret_src: Any.t)
                       (WLE: le a0 a1)
-                      ctx1
-                      (ACC: current_iPropL ctx1 ((Invn, R a1 mp_src1 mp_tgt1) :: (Rn, fsp1.(postcond) x vret_src vret_tgt) :: snd (alist_pops Hns l)))
+                      fr1
+                      (ACC: current_iPropL (fr1 ⋅ mr_src1) ((Invn, R a1 mp_src1 mp_tgt1) :: (Rn, fsp1.(postcond) x vret_src vret_tgt) :: snd (alist_pops Hns l)))
           ,
             gpaco8 (_sim_itree (mk_wf R) le fl_src fl_tgt) (cpn8 (_sim_itree (mk_wf R) le fl_src fl_tgt)) rg rg _ _ eqr true true a
-                   ((Any.pair mp_src1 mr_src1↑), k_src (ctx1, vret_src)) (mp_tgt1, k_tgt vret_tgt))
+                   ((Any.pair mp_src1 mr_src1↑), k_src (fr1, vret_src)) (mp_tgt1, k_tgt vret_tgt))
     :
       gpaco8 (_sim_itree (mk_wf R) le fl_src fl_tgt) (cpn8 (_sim_itree (mk_wf R) le fl_src fl_tgt)) r rg _ _ eqr m n a
-             ((Any.pair mp_src0 mr_src0), (HoareCall tbr ord_cur fsp0 fn varg_src) ctx0 >>= k_src)
+             ((Any.pair mp_src0 mr_src0↑), (HoareCall tbr ord_cur fsp0 fn varg_src) fr0 >>= k_src)
              (mp_tgt0, trigger (Call fn varg_tgt) >>= k_tgt)
   .
   Proof.
@@ -369,8 +373,8 @@ Section HLEMMAS.
 
         (WEAKER: fspec_weaker fsp1 fsp0)
 
-        ctx0 l
-        (ACC: current_iPropL ctx0 l)
+        fr0 l
+        (ACC: current_iPropL (fr0 ⋅ mr_src0) l)
 
         (UPDATABLE:
            from_iPropL (fst (alist_pops Hns l)) ⊢ #=> (R a0 mp_src0 mp_tgt0 ** (fsp1.(precond) x varg_src varg_tgt: iProp)))
@@ -381,14 +385,14 @@ Section HLEMMAS.
         (POST: forall (vret_tgt : Any.t) (mr_src1: Σ) mp_src1 mp_tgt1 a1
                       (vret_src: Any.t)
                       (WLE: le a0 a1)
-                      ctx1
-                      (ACC: current_iPropL ctx1 (@cons (prod string (bi_car iProp)) (Invn, R a1 mp_src1 mp_tgt1) (@cons (prod string (bi_car iProp)) (Rn, fsp1.(postcond) x vret_src vret_tgt) (snd (alist_pops Hns l)))))
+                      fr1
+                      (ACC: current_iPropL (fr1 ⋅ mr_src1) (@cons (prod string (bi_car iProp)) (Invn, R a1 mp_src1 mp_tgt1) (@cons (prod string (bi_car iProp)) (Rn, fsp1.(postcond) x vret_src vret_tgt) (snd (alist_pops Hns l)))))
           ,
             gpaco8 (_sim_itree (mk_wf R) le fl_src fl_tgt) (cpn8 (_sim_itree (mk_wf R) le fl_src fl_tgt)) rg rg _ _ eqr true true a
-                   ((Any.pair mp_src1 mr_src1↑), k_src (ctx1, vret_src)) (mp_tgt1, k_tgt vret_tgt))
+                   ((Any.pair mp_src1 mr_src1↑), k_src (fr1, vret_src)) (mp_tgt1, k_tgt vret_tgt))
     :
       gpaco8 (_sim_itree (mk_wf R) le fl_src fl_tgt) (cpn8 (_sim_itree (mk_wf R) le fl_src fl_tgt)) r rg _ _ eqr m n a
-             ((Any.pair mp_src0 mr_src0), (HoareCall tbr ord_cur fsp0 fn varg_src) ctx0 >>= k_src)
+             ((Any.pair mp_src0 mr_src0↑), (HoareCall tbr ord_cur fsp0 fn varg_src) fr0 >>= k_src)
              (mp_tgt0, trigger (Call fn varg_tgt) >>= k_tgt)
   .
   Proof.
@@ -409,8 +413,8 @@ Section HLEMMAS.
         (R: A -> Any.t -> Any.t -> iProp)
         (eqr: Any.t -> Any.t -> Any.t -> Any.t -> Prop)
 
-        ctx0 l
-        (ACC: current_iPropL ctx0 l)
+        fr0 l
+        (ACC: current_iPropL (fr0 ⋅ mr_src0) l)
 
         (UPDATABLE:
            from_iPropL (fst (alist_pops Hns l)) ⊢ #=> (R a0 mp_src0 mp_tgt0 ** (P x varg_src varg_tgt: iProp)))
@@ -421,14 +425,14 @@ Section HLEMMAS.
         (POST: forall (vret_tgt : Any.t) (mr_src1: Σ) mp_src1 mp_tgt1 a1
                       (vret_src: Any.t)
                       (WLE: le a0 a1)
-                      ctx1
-                      (ACC: current_iPropL ctx1 (@cons (prod string (bi_car iProp)) (Invn, R a1 mp_src1 mp_tgt1) (@cons (prod string (bi_car iProp)) (Rn, Q x vret_src vret_tgt) (snd (alist_pops Hns l)))))
+                      fr1
+                      (ACC: current_iPropL (fr1 ⋅ mr_src1) (@cons (prod string (bi_car iProp)) (Invn, R a1 mp_src1 mp_tgt1) (@cons (prod string (bi_car iProp)) (Rn, Q x vret_src vret_tgt) (snd (alist_pops Hns l)))))
           ,
                 gpaco8 (_sim_itree (mk_wf R) le fl_src fl_tgt) (cpn8 (_sim_itree (mk_wf R) le fl_src fl_tgt)) rg rg _ _ eqr true true a
-                       ((Any.pair mp_src1 mr_src1↑), k_src (ctx1, vret_src)) (mp_tgt1, k_tgt vret_tgt))
+                       ((Any.pair mp_src1 mr_src1↑), k_src (fr1, vret_src)) (mp_tgt1, k_tgt vret_tgt))
     :
       gpaco8 (_sim_itree (mk_wf R) le fl_src fl_tgt) (cpn8 (_sim_itree (mk_wf R) le fl_src fl_tgt)) r rg _ _ eqr m n a
-             ((Any.pair mp_src0 mr_src0), (HoareCall tbr ord_cur (mk_fspec D P Q) fn varg_src) ctx0 >>= k_src)
+             ((Any.pair mp_src0 mr_src0↑), (HoareCall tbr ord_cur (mk_fspec D P Q) fn varg_src) fr0 >>= k_src)
              (mp_tgt0, trigger (Call fn varg_tgt) >>= k_tgt)
   .
   Proof.
@@ -451,10 +455,10 @@ Section HLEMMAS.
         m n
         (ARG:
            forall x varg_src
-                  ctx (mr_src: Σ) mp_src
-                  (ACC: current_iPropL ctx (@cons (prod string (bi_car iProp)) (Rn, P  x varg_src varg) (@cons (prod string (bi_car iProp)) (Invn, R a mp_src mp_tgt) (@nil (prod string (bi_car iProp)))))),
+                  fr0 (mr_src: Σ) mp_src
+                  (ACC: current_iPropL (fr0 ⋅ mr_src) (@cons (prod string (bi_car iProp)) (Rn, P  x varg_src varg) (@cons (prod string (bi_car iProp)) (Invn, R a mp_src mp_tgt) (@nil (prod string (bi_car iProp)))))),
              gpaco8 (_sim_itree (mk_wf R) le fl_src fl_tgt) (cpn8 (_sim_itree (mk_wf R) le fl_src fl_tgt)) r rg _ _  eqr true n a
-                    ((Any.pair mp_src mr_src↑), k_src (ctx, (x, varg_src)))
+                    ((Any.pair mp_src mr_src↑), k_src (fr0, (x, varg_src)))
                     (mp_tgt, f_tgt))
     :
       gpaco8 (_sim_itree (mk_wf R) le fl_src fl_tgt) (cpn8 (_sim_itree (mk_wf R) le fl_src fl_tgt)) r rg _ _  eqr m n a
@@ -463,20 +467,19 @@ Section HLEMMAS.
   .
   Proof.
     inv WF.
-    unfold HoareFunArg, ASSUME, ASSERT, mput, mget, assume, guarantee.
+    unfold HoareFunArg,  mput, mget, assume, guarantee.
     repeat (ired_both; apply sim_itreeC_spec; econs). intro x.
-    repeat (ired_both; apply sim_itreeC_spec; econs). intros (rarg_src, ctx).
+    repeat (ired_both; apply sim_itreeC_spec; econs). intros varg_src.
+    repeat (ired_both; apply sim_itreeC_spec; econs). intros rarg_src.
     repeat (ired_both; apply sim_itreeC_spec; econs). intros VALID.
-    repeat (ired_both; apply sim_itreeC_spec; econs). intro varg_src.
     repeat (ired_both; apply sim_itreeC_spec; econs). intro PRE.
     ired_both. eapply ARG; et.
-    red. econs.
-    { instantiate (1:=rarg_src ⋅ ε ⋅ mr_src). r_wf VALID. }
+    red. econs; ss; cycle 1.
+    { instantiate (1:=rarg_src ⋅ mr_src). refl. }
     { ss. rr. uipropall. esplits; et.
       { rewrite URA.unit_id. et. }
-      2: { eapply RSRC; et. eapply URA.wf_mon. instantiate (1:=(ctx ⋅ rarg_src)). r_wf VALID. }
-      { rewrite URA.unit_id. ss. }
-      { rr. uipropall. }
+      { eapply RSRC; et. eapply URA.wf_mon. instantiate (1:=(rarg_src)). r_wf VALID. }
+            { rr. uipropall. }
     }
   Qed.
 
@@ -490,8 +493,8 @@ Section HLEMMAS.
         (eqr: Any.t -> Any.t -> Any.t -> Any.t -> Prop)
         (R: A -> Any.t -> Any.t -> iProp)
 
-        ctx l
-        (ACC: current_iPropL ctx l)
+        fr0 l
+        (ACC: current_iPropL (fr0 ⋅ mr_src) l)
 
         (WLE: le a0 a)
 
@@ -502,28 +505,27 @@ Section HLEMMAS.
             eqr ((Any.pair mp_src mr_src1↑)) mp_tgt vret_tgt vret_tgt)
     :
       gpaco8 (_sim_itree (mk_wf R) le fl_src fl_tgt) (cpn8 (_sim_itree (mk_wf R) le fl_src fl_tgt)) r rg _ _  eqr m n a0
-             ((Any.pair mp_src mr_src), (HoareFunRet Q x (ctx, vret_src)))
+             ((Any.pair mp_src mr_src↑), (HoareFunRet Q x (fr0, vret_src)))
              (mp_tgt, (Ret vret_tgt))
   .
   Proof.
-    subst. unfold HoareFunRet, ASSUME, ASSERT, mput, mget, guarantee.
+    subst. unfold HoareFunRet, mput, mget, guarantee.
+    repeat (ired_both; apply sim_itreeC_spec; econs). exists vret_tgt.
+    repeat (ired_both; apply sim_itreeC_spec; econs).
     assert (exists mr_src1 rret_src,
-               (<<UPDATABLE: URA.wf (ctx ⋅ (mr_src1 ⋅ rret_src))>>) /\
+               (<<UPDATABLE: URA.updatable (fr0 ⋅ mr_src) (mr_src1 ⋅ rret_src)>>) /\
                (<<RSRC: R a mp_src mp_tgt mr_src1>>) /\
                (<<PRE: Q  x vret_src vret_tgt rret_src>>)).
     { red in ACC. inv ACC. uipropall.
       hexploit (UPDATABLE r0); et.
-      { eapply URA.wf_mon; et. }
+      { eapply URA.updatable_wf; et. }
       i. des. subst. exists a1, b. splits; et.
-      replace (ctx ⋅ (a1 ⋅ b)) with (a1 ⋅ b ⋅ ctx); et.
-      r_solve.
+      etrans; et.
     }
-    des.
-    repeat (ired_both; apply sim_itreeC_spec; econs). exists (rret_src, ε, mr_src1).
+    des. exists (rret_src, ε, mr_src1).
     repeat (ired_both; apply sim_itreeC_spec; econs). unshelve esplits.
-    { r_wf UPDATABLE0. }
-    repeat (ired_both; apply sim_itreeC_spec; econs). exists vret_tgt.
-    repeat (ired_both; apply sim_itreeC_spec; econs). unshelve esplits; eauto.
+    { rewrite URA.unit_id. replace (rret_src ⋅ mr_src1) with (mr_src1 ⋅ rret_src) by r_solve. ss. }
+    repeat (ired_both; apply sim_itreeC_spec; econs). unshelve esplits; et.
     repeat (ired_both; apply sim_itreeC_spec; econs).
     eapply EQ; et. econs; et.
   Qed.
